investigations/bedrock2/Aes/Aes.v
@@ -6,6 +6,7 @@ Require Import bedrock2.Syntax.
 Require Import bedrock2.NotationsCustomEntry.
 Require Import bedrock2.ToCString.
 Require Import coqutil.Word.Interface.
+Require Import Bedrock2Experiments.LibBase.MMIOLabels.
 Require Import Bedrock2Experiments.StateMachineSemantics.
 Require Import Bedrock2Experiments.Aes.Constants.
 Require Import Bedrock2Experiments.Aes.AesSemantics.
@@ -51,7 +52,7 @@ Section Impl.
      ([aes_cfg_operation; aes_cfg_mode; aes_cfg_key_len;
       aes_cfg_manual_operation],
       [], bedrock_func_body:(
-      output! WRITE (AES_CTRL0,
+      output! WRITE32 (AES_CTRL0,
                      ((aes_cfg_operation << AES_CTRL_OPERATION) |
                       ((aes_cfg_mode & AES_CTRL_MODE_MASK)
                          << AES_CTRL_MODE_OFFSET) |
@@ -103,13 +104,13 @@ Section Impl.
 
       i = 0 ;
       while (i < num_regs_key_used) {
-        output! WRITE (AES_KEY00 + (i * 4), load4(key + (i * 4)));
+        output! WRITE32 (AES_KEY00 + (i * 4), load4(key + (i * 4)));
         i = i + 1
       };
 
       i = num_regs_key_used ;
       while (i < AES_NUM_REGS_KEY) {
-        output! WRITE (AES_KEY00 + (i * 4), 0);
+        output! WRITE32 (AES_KEY00 + (i * 4), 0);
         i = i + 1
       }
     ))).
@@ -129,7 +130,7 @@ Section Impl.
      ([iv], [], bedrock_func_body:(
       i = 0 ;
       while (i < AES_NUM_REGS_IV) {
-        output! WRITE (AES_IV00 + (i * 4), load4( iv + (i * 4) ));
+        output! WRITE32 (AES_IV00 + (i * 4), load4( iv + (i * 4) ));
         i = i + 1
       }
     ))).
@@ -150,7 +151,7 @@ Section Impl.
       bedrock_func_body:(
       i = 0 ;
       while (i < AES_NUM_REGS_DATA) {
-        output! WRITE (AES_DATA_IN00 + (i * 4), load4( data + (i * 4) ));
+        output! WRITE32 (AES_DATA_IN00 + (i * 4), load4( data + (i * 4) ));
         i = i + 1
       }
     ))).
@@ -172,7 +173,7 @@ Section Impl.
       bedrock_func_body:(
       i = 0 ;
       while (i < AES_NUM_REGS_DATA) {
-        io! val = READ ( AES_DATA_OUT00 + (i * 4) ) ;
+        io! val = READ32 ( AES_DATA_OUT00 + (i * 4) ) ;
         store4( data + (i * 4), val ) ; (* data[i] = val *)
         i = i + 1
       }
@@ -189,7 +190,7 @@ Section Impl.
     ("b2_data_ready",
      ([], [out],
       bedrock_func_body:(
-      io! status = READ (AES_STATUS0) ;
+      io! status = READ32 (AES_STATUS0) ;
       out = status & (1 << AES_STATUS_INPUT_READY)
     ))).
 
@@ -204,7 +205,7 @@ Section Impl.
     ("b2_data_valid",
      ([], [out],
       bedrock_func_body:(
-      io! status = READ (AES_STATUS0) ;
+      io! status = READ32 (AES_STATUS0) ;
       out = status & (1 << AES_STATUS_OUTPUT_VALID)
     ))).
 
@@ -219,7 +220,7 @@ Section Impl.
     ("b2_idle",
      ([], [out],
       bedrock_func_body:(
-      io! status = READ (AES_STATUS0) ;
+      io! status = READ32 (AES_STATUS0) ;
       out = status & (1 << AES_STATUS_IDLE)
     ))).
 
